src/lib/data/Kuiper.Array1.fsti
@@ -131,7 +131,8 @@ fn alloc0
   ensures
     exists* em. on gpu_loc (p |-> em)
   ensures
-    pure (is_global p)
+    pure (is_global p) **
+    pure (is_full_array (core p))
 
 inline_for_extraction noextract
 fn free
@@ -143,7 +144,8 @@ fn free
   preserves
     cpu
   requires
-    on gpu_loc (p |-> em)
+    on gpu_loc (p |-> em) **
+    pure (is_full_array (core p))
   ensures
     emp
 
