src/lib/data/Kuiper.Tensor.fsti
@@ -93,7 +93,8 @@ fn alloc0
   ensures
     exists* em. on gpu_loc (p |-> em)
   ensures
-    pure (is_global p)
+    pure (is_global p) **
+    pure (is_full_array (core p))
 
 inline_for_extraction noextract
 fn free
@@ -105,6 +106,7 @@ fn free
   preserves
     cpu
   requires
+    pure (is_full_array (core p)) **
     on gpu_loc (p |-> em)
   ensures emp
 
